src/usuba_AST.v
@@ -3,6 +3,9 @@ Require Import Coq.NArith.NArith.
 Require Import List.
 Import ListNotations.
 
+Require Import Coq.FSets.FMapPositive.
+Module PM := Coq.FSets.FMapPositive.PositiveMap.
+
 
 Require Import Coq.extraction.ExtrOcamlBasic.
 Require Import Coq.extraction.ExtrOcamlZInt.
@@ -12,45 +15,73 @@ Require Import Coq.extraction.ExtrOcamlString.
 (* XXX: this won't work for actual extraction*)
 Extract Inductive string => "string"  [ """" "^" ].
 
+(*################################################################*)
+(* Identifiers *)
+
 Record ident := { uid: positive;
                   name: string }.
+
+(*################################################################*)
+(* Types *)
+
+Inductive typ :=
+  (* [[Atom k]] is a machine word of size [[k]] *)
+  | ATOM: nat -> typ
+  (* [[TUP tys]] is an heterogeneous list *)
+  | TUP (t: list typ).
+  (* XXX: I don't understand these: *)
+  (* | Int (i: N) (j :N) *)
+  (* | Nat (* for recurrence variables. Not part of usuba0 normalized *) *)
+  (* | Array (t: typ)(ae: arith_expr) (* arrays *) *)
+
+(*################################################################*)
+(* Clocks *)
+
 Inductive clock :=
 | Defclock (* Temporary, for clocks we don't know *)
 | Base
 | On (ck:clock) (x:ident)
 | Onot (ck:clock) (x:ident).
 
-Inductive log_op := And | Or | Xor | Andn.
+(*################################################################*)
+(* Values *)
+
+Inductive val :=
+| Atom: nat -> N -> val (* N.size_nat n < k *)
+| Tup: list val -> val.
+
+Definition Ttrue := Atom 1 1%N.
+Definition Tfalse := Atom 1 0%N.
+
+(*################################################################*)
+(* Compile-time expressions *)
+
 Inductive arith_op := Add | Mul | Sub | Div | Mod.
-Inductive shift_op := Lshift | Rshift | Lrotate | Rrotate.
 
 Inductive arith_expr :=
   | Const_e (i: N)
   | Var_e (x: ident)
-  | Op_e (op: arith_op)(e1 e2: arith_expr). 
+  | Op_e (op: arith_op)(e1 e2: arith_expr).
 
-Inductive typ :=
-  | Bool
-  | Int (i: N) (j :N)
-  | Nat (* for recurrence variables. Not part of usuba0 normalized *)
-  | Array (t: typ)(ae: arith_expr). (* arrays *)
-
-Inductive constr :=
-  | True
-  | False.
+(*################################################################*)
+(* Run-time expressions *)
 
 Inductive var :=
   | Var (i: ident)
-(* XXX: update the rest of the code so that it takes a [var] and not an [ident]  *)
+  (* XXX: update the rest of the code so that it takes a [var] and not an [ident]  *)
   | Slice (v: var)(aes: list arith_expr)
   | Range (v: var)(ae1 ae2: arith_expr).
 
 Definition Field (v: var)(ae: arith_expr) := Slice v [ae].
 Definition Index (x: ident)(ae: arith_expr) := Slice (Var x) [ae].
 
+
+Inductive log_op := And | Or | Xor | Andn.
+Inductive shift_op := Lshift | Rshift | Lrotate | Rrotate.
+
 (* XXX: factorize operations in a single case *)
 Inductive expr :=
-  | Const (i: N)
+  | Const (v: val)
   | ExpVar (v: var)
   | Tuple (es: list expr)
   | Not (e: expr) (* special case for bitwise not *)
@@ -58,26 +89,32 @@ Inductive expr :=
   | Log  (op: log_op)(e1 e2: expr)
   | Fun (x: ident)(es: list expr)
   (* XXX: not yet supported by the semantics *)
-  | Fun_v (x: ident)(ae: arith_expr)(es: list expr) (* nodes arrays *)
+(*  | Fun_v (x: ident)(ae: arith_expr)(es: list expr) (* nodes arrays *) *)
   (* XXX: not yet supported by the semantics *)
-  | When (e: expr)(x: constr) (y: ident)
+(*  | When (e: expr)(x: constr) (y: ident) *)
   (* XXX: not yet supported by the semantics *)
-  | Merge (x: ident)(xs: list (constr * expr))
+(*  | Merge (x: ident)(xs: list (constr * expr)) *)
   (* XXX: how could we bitslice an arithmetic operation (efficiently)? *)
-  | Arith (op: arith_op)(e1 e2: expr)
+(*  | Arith (op: arith_op)(e1 e2: expr) *)
   (* XXX: we do not actually support fby *)
-  | Fby (e1 e2: expr)(mx: option ident).
+(*  | Fby (e1 e2: expr)(mx: option ident) *).
 
 Inductive deq :=
   | Norec (vs: list var)(e: expr)
+  (* XXX: what is the meaning of [x]? *)
   | Rec (x: ident)(ae1 ae2: arith_expr)(dl: list deq).
 
-(* XXX: define a record for [ident * typ * clock] *)
-Definition p := list (ident * typ * clock).
+Record formal := { t : typ ;
+                   c : clock }.
+Definition formals := list (ident * formal).
+
+Definition vars_of (p: formals): list ident := map fst p.
+Definition typs_of (p: formals): list typ := map (fun x => (snd x).(t)) p.
+
 
 Inductive def_i :=
-  | Single        (n: p)(ds: list deq) (* regular node *)
-  | Multiple      (an: list (p * list deq)) (*array of nodes*)
+  | Single        (locals: formals)(ds: list deq) (* regular node *)
+  | Multiple      (an: list (formals * list deq)) (*array of nodes*)
   | Perm          (pi: list N) (* permutation *)
   | MultiplePerm  (pis: list (list N)) (* array of perm *)
   | Table         (t: list N) (* lookup table *)
@@ -86,16 +123,14 @@ Inductive def_i :=
 Inductive def_opt := Inline | No_inline.
 
 Record def := {
-  id    : ident;
-  p_in  : p;
-  p_out : p;
+  d_name: string;
+  p_in  : formals;
+  p_out : formals;
   opt   : list def_opt;
   node  : def_i;
 }.
 
-Record prog := {
-  nodes : list def;
-}.
+Definition prog := list (ident * def).
 
 
 Inductive arch :=
@@ -135,6 +170,6 @@ Record config := {
 
 Set Extraction KeepSingleton.
 Extraction "usuba_AST.ml" 
-           config prog def def_opt def_i p deq
+           config prog def def_opt def_i formals deq
            expr var typ arith_expr shift_op
            arith_op log_op clock ident arch.
