src/lib.v
@@ -1,0 +1,144 @@
+Require Import Coq.NArith.NArith.
+
+Require Import List.
+Import ListNotations.
+
+
+(* XXX: lengthy prelude *)
+
+Definition fmap {A B} (f: A -> B)(x: option A) : option B :=
+  match x with
+  | None => None
+  | Some i => Some (f i)
+  end.
+
+Definition bind {A B} (x: option A)(f : A -> option B): option B :=
+  match x with
+  | None => None
+  | Some i => f i
+  end.
+
+Notation "'let!' x ':=' ma 'in' f" :=
+  (bind ma (fun x => f))
+    (at level 200, right associativity).
+
+Notation "'ret!' x" := (Some x)
+                         (at level 200).
+
+Notation "'fail!'" := (None)
+                         (at level 200).
+
+
+Fixpoint pos_to_list (k: nat)(p: positive): list bool :=
+  match k with
+  | 0 => []
+  | S k =>
+    match p with
+    | xI p => true :: pos_to_list k p
+    | xO p => false :: pos_to_list k p
+    | xH => true :: repeat false k
+    end
+  end.
+
+Definition to_list (k: nat)(n: N): list bool :=
+  match n with
+  | N0 => repeat false k
+  | Npos p => pos_to_list k p
+  end.
+
+Lemma test__to_list15: to_list 8 12 =
+                       [false; false; true; true; false; false; false; false].
+Proof. trivial. Qed.
+
+Definition lnand (k: nat) (x y: N): N := N.lnot (N.land x y) (N.of_nat k).
+
+Definition rotl {A}(n: nat)(l: list A) :=
+  skipn n l ++ firstn n l.
+
+Definition rotr {A}(n: nat)(l: list A) :=
+  rotl (length l - n) l.
+
+Definition shl {A}(n: nat)(d: A)(l: list A): list A :=
+  skipn n l ++ repeat d (min n (length l)).
+
+Definition shr {A}(n: nat)(d: A)(l: list A): list A :=
+  repeat d (min n (length l)) ++ firstn (length l - n) l.
+
+Lemma test__Lshift0: shl 0 0 [1; 2; 3; 4; 5] = [1; 2; 3; 4; 5].
+Proof. trivial. Qed.
+
+Lemma test__Lshift1: shl 1 0 [1; 2; 3; 4; 5] = [2; 3; 4; 5; 0].
+Proof. trivial. Qed.
+
+Lemma test__Lshift5: shl 5 0 [1; 2; 3; 4; 5] = [0; 0; 0; 0; 0].
+Proof. trivial. Qed.
+
+Lemma test__Lshift6: shl 6 0 [1; 2; 3; 4; 5] = [0; 0; 0; 0; 0].
+Proof. trivial. Qed.
+
+Lemma test__Rshift1: shr 1 0 [1; 2; 3; 4; 5] = [0; 1; 2; 3; 4].
+Proof. trivial. Qed.
+
+Lemma test__Rshift5: shr 5 0 [1; 2; 3; 4; 5] = [0; 0; 0; 0; 0].
+Proof. trivial. Qed.
+
+Lemma test__Rshift6: shr 6 0 [1; 2; 3; 4; 5] = [0; 0; 0; 0; 0].
+Proof. trivial. Qed.
+
+
+Lemma test__Lrotate0: rotl 0 [1; 2; 3; 4; 5] = [1; 2; 3; 4; 5].
+Proof. trivial. Qed.
+
+Lemma test__Lrotate1: rotl 1 [1; 2; 3; 4; 5] = [2; 3; 4; 5; 1].
+Proof. trivial. Qed.
+
+Lemma test__Lrotate4: rotl 4 [1; 2; 3; 4; 5] = [5; 1; 2; 3; 4].
+Proof. trivial. Qed.
+
+Lemma test__Lrotate5: rotl 5 [1; 2; 3; 4; 5] = [1; 2; 3; 4; 5].
+Proof. trivial. Qed.
+
+Lemma test__Lrotate6: rotl 6 [1; 2; 3; 4; 5] = [1; 2; 3; 4; 5].
+Proof. trivial. Qed.
+
+Lemma test__Rrotate1: rotr 1 [1; 2; 3; 4; 5] = [5; 1; 2; 3; 4].
+Proof. trivial. Qed.
+
+Lemma test__Rrotate4: rotr 4 [1; 2; 3; 4; 5] = [2; 3; 4; 5; 1].
+Proof. trivial. Qed.
+
+Lemma test__Rrotate5: rotr 5 [1; 2; 3; 4; 5] = [1; 2; 3; 4; 5].
+Proof. trivial. Qed.
+
+Lemma test__Rrotate6: rotr 6 [1; 2; 3; 4; 5] = [1; 2; 3; 4; 5].
+Proof. trivial. Qed.
+
+
+Fixpoint mask {A}(l: list A)(k1 k2: nat): option (list A) :=
+  match k2 with
+  | 0 => ret! []
+  | S k2 =>
+    match k1 with
+    | S k1 => match l with
+             | [] => fail!
+             | x :: xs => mask xs k1 k2
+             end
+    | 0 => match l with
+          | [] => fail!
+          | x :: xs =>
+            let! xs := mask xs 0 k2 in
+            ret! (x :: xs)
+          end
+    end
+  end.
+
+Lemma test__mask: mask [0; 1; 2; 3; 4; 5; 6; 7] 2 5 = Some [2; 3; 4].
+Proof. auto. Qed.
+
+
+
+
+Inductive Forall3 {A B C : Type} (R : A -> B -> C -> Prop) : list A -> list B -> list C -> Prop :=
+    Forall3_nil : Forall3 R [] [] []
+  | Forall3_cons : forall (x : A) (y : B)(z : C) (l : list A) (l' : list B)(l'' : list C),
+                   R x y z -> Forall3 R l l' l'' -> Forall3 R (x :: l) (y :: l') (z :: l'').
