src/usuba_correctness.v
@@ -1,0 +1,35 @@
+Require Import Coq.FSets.FMapPositive.
+Module PM := Coq.FSets.FMapPositive.PositiveMap.
+
+Require Import Coq.NArith.NArith.
+Require Import List.
+Import ListNotations.
+
+Require Import usuba_AST.
+Require Import usuba_sem.
+Require Import usuba_typing.
+
+Lemma sem_exists0: forall prog f fnode ins,
+    (* the graph of nodes is well-founded: *)
+(*    dependency prog -> *)
+    (* the graph of equations in each nodes is well-founded: *)
+(*    sch_prog prog -> *)
+    (* the program is well-typed: *)
+    ty_prog prog ->
+    In (f, fnode) prog ->
+    (* the input values are well-typed: *)
+    Forall2 ty_val ins (typs_of fnode.(p_in)) ->
+    exists outs,
+        Forall2 ty_val outs (typs_of fnode.(p_out))
+     /\ sem_node prog fnode ins outs.
+Admitted.
+
+Theorem sem_exists: forall prog f fnode ins,
+    ty_prog prog ->
+    In (f, fnode) prog ->
+    Forall2 ty_val ins (typs_of fnode.(p_in)) ->
+    exists outs,
+      sem_node prog fnode ins outs.
+Proof.
+(* By generalization sem_exists0 *)
+Admitted.
