src/usuba_typing.v
@@ -1,0 +1,98 @@
+Require Import Coq.FSets.FMapPositive.
+Module PM := Coq.FSets.FMapPositive.PositiveMap.
+
+Require Import Coq.NArith.NArith.
+Require Import List.
+Import ListNotations.
+
+Require Import usuba_AST.
+
+Definition context := PM.t typ.
+
+Inductive ty_var: context -> var -> typ -> Prop :=
+  | ty_Var: forall ctxt i ty,
+      PM.find (uid i) ctxt = Some ty ->
+      ty_var ctxt (Var i) ty.
+  (* XXX: TODO *)
+(*
+  | ty_Slice: forall ctxt v aes ty,
+      False -> ty_var ctxt (Slice v aes) ty
+  | ty_Range: forall ctxt v ae1 ae2 ty,
+      False -> ty_var ctxt (Range v ae1 ae2) ty
+*)
+
+Section TypeExpr.
+
+Variable prog: list (ident * def).
+
+Definition get_def : ident -> option def.
+Admitted.
+
+Inductive ty_val: val -> typ -> Prop :=
+  | ty_Tup: forall vs tys,
+      Forall2 ty_val vs tys ->
+      ty_val (Tup vs) (TUP tys)
+  | ty_Atom: forall k n,
+      N.size_nat n < k ->
+      ty_val (Atom k n) (ATOM k).
+
+Inductive ty_expr: context -> expr -> typ -> Prop :=
+  | ty_Const: forall ctxt v ty,
+      ty_val v ty ->
+      ty_expr ctxt (Const v) ty
+  | ty_ExpVar: forall ctxt v ty,
+      ty_var ctxt v ty ->
+      ty_expr ctxt (ExpVar v) ty
+  | ty_Tuple: forall ctxt es tys,
+      Forall2 (ty_expr ctxt) es tys ->
+      ty_expr ctxt (Tuple es) (TUP tys)
+  | ty_Not: forall ctxt e ty,
+      (* XXX: Not applies to anything, pointwise *)
+      ty_expr ctxt e ty ->
+      ty_expr ctxt (Not e) ty
+  | ty_Shift: forall ctxt op e ae tys tys',
+      ty_expr ctxt e (TUP tys) ->
+      (* XXX: apply shift on tys, gives tys' *)
+      ty_expr ctxt (Shift op e ae) (TUP tys')
+  | ty_Log: forall ctxt op e1 e2 ty,
+      ty_expr ctxt e1 ty ->
+      ty_expr ctxt e2 ty ->
+      (* XXX: Logical operations apply to anything, pointwise *)
+      ty_expr ctxt (Log op e1 e2) ty
+  | ty_Fun: forall ctxt x es def,
+      get_def x = Some def ->
+      Forall2 (ty_expr ctxt) es (typs_of def.(p_in)) ->
+      ty_expr ctxt (Fun x es) (TUP (typs_of def.(p_out))).
+(*
+  | ty_Arith: forall ctxt op e1 e2 ty,
+      ty_expr ctxt e1 ty ->
+      ty_expr ctxt e2 ty ->
+      (* XXX: only a few types support arithmetic operations *)
+      ty_expr ctxt (Arith_op e1 e2) ty.
+*)
+
+Fixpoint ctxt_of (x: formals): PM.t typ :=
+  match x with
+  | [] => PM.empty _
+  | (x, formal) :: xs => PM.add (uid x) formal.(t) (ctxt_of xs)
+  end.
+
+Inductive ty_deq: context -> deq -> Prop :=
+  | ty_Norec : forall ctxt vs e tys,
+      Forall2 (ty_var ctxt) vs tys ->
+      ty_expr ctxt e (TUP tys) ->
+      ty_deq ctxt (Norec vs e).
+
+Definition ty_node (d: def): Prop :=
+  match d.(node) with
+  | Single n ds =>
+    let ctxt := ctxt_of (d.(p_in) ++ d.(p_out) ++ n) in
+    Forall (ty_deq ctxt) ds
+  | _ => False
+  end.
+
+End TypeExpr.
+
+Definition ty_prog (p: prog): Prop :=
+  (* XXX: this does not forbid self-definition *)
+  forall x d, In (x, d) p -> ty_node p d.
